Envelope example

theories/Thomas.v
@@ -904,4 +904,301 @@ Module Thomas.
        blast_cases; simpl in *; kill Heqm; simpl in *.
        all: bs.
   Qed.
+
+
+  Notation "'let?' x := service '!' arg 'in' cont" :=
+    (h_call service arg (fun x => cont))
+      ( x pattern,
+        at level 61,
+        right associativity,
+        service at next level,
+        arg at next level
+      ).
+
+  Notation reply := h_reply.
+
+  Section Example.
+    Definition echo := worker_conf tt (fun _from msg st => reply msg st).
+
+    Definition proxy (target : string) :=
+      worker_conf tt (fun _from msg st => let? v' := target ! msg in reply v' st).
+
+    Definition endpoint (target : string) :=
+      let handle_call (from : Name) (msg : Val) st :=
+        match from with
+        | Initiator _ _ =>
+            let? v' := target ! msg in
+            reply v' st
+        | _ => reply msg st
+        end
+      in worker_conf tt handle_call.
+
+    Definition echo_proxy (target : string) :=
+      let init_state := false in
+      let handle_call (from : Name) (msg : Val) (activated : bool) :=
+        if activated
+        then
+          let? v' := target ! msg in
+          reply v' true
+        else
+          reply msg true
+      in worker_conf init_state handle_call.
+
+    Variable some_msg : Payload.
+
+    Definition my_net_conf : NetConf :=
+      {| workers name :=
+          match name with
+          | "endpoint0" => endpoint "proxy1"
+          | "endpoint1" => endpoint "proxy0"
+          | "proxy0" => proxy "endpoint0"
+          | "proxy1" => proxy "endpoint1"
+          | _ => echo (* We default to echo *)
+          end;
+
+        inits name :=
+          match name with
+          | "0" => init_conf "endpoint0" (some_msg : Val)
+          | "1" => init_conf "endpoint1" (some_msg : Val)
+          | _ => init_conf "" (some_msg : Val) (* Default *)
+          end
+      |}.
+
+  Lemma ded : exists path N, (make_net my_net_conf =[path]=> N) /\ Deadlocked N.
+  Proof.
+    eexists ?[path], ?[N].
+
+    eassert ((make_net my_net_conf =[?path]=> ?N)).
+    {
+      (* Session 0 *)
+      eapply path_seq1 with (act := NTau (Initiator "0" 0) Tau).
+      {
+        unfold make_net, my_net_conf, call, recvr, recvq.
+        repeat econstructor.
+        rewrite NetMod.init_get.
+        eattac.
+      }
+
+      eapply path_seq1 with (act := NComm (Initiator "0" 0) (Worker "endpoint0") Q some_msg).
+      {
+        unfold make_net, my_net_conf, call, recvr, recvq.
+        eapply NComm_neq; eattac.
+        - repeat econstructor.
+          compat_hsimpl in *.
+          eattac.
+        - repeat econstructor.
+          compat_hsimpl in *.
+          rewrite NetMod.init_get.
+          eattac.
+      }
+
+      eapply path_seq1 with (act := NTau (Worker "endpoint0") Tau).
+      {
+        unfold make_net, my_net_conf, call, recvr, recvq.
+        rewrite (unfold_Proc (gen_server _ _)).
+        simpl.
+        repeat econstructor.
+        compat_hsimpl.
+        eattac.
+      }
+
+      eapply path_seq1 with (act := NTau (Worker "endpoint0") Tau).
+      {
+        unfold make_net, my_net_conf, call, recvr, recvq.
+        rewrite (unfold_Proc (run_gen_server _)); simpl.
+        repeat econstructor.
+        compat_hsimpl.
+        eattac.
+      }
+
+      eapply path_seq1 with (act := NComm (Worker "endpoint0") (Worker "proxy1") Q some_msg).
+      {
+        unfold make_net, my_net_conf, call, recvr, recvq.
+        eapply NComm_neq; eattac.
+        - repeat econstructor.
+          compat_hsimpl in *.
+          eattac.
+        - repeat econstructor.
+          compat_hsimpl in *.
+          rewrite NetMod.init_get.
+          eattac.
+      }
+
+      (* Session 1 *)
+      eapply path_seq1 with (act := NTau (Initiator "1" 0) Tau).
+      {
+        unfold make_net, my_net_conf, call, recvr, recvq.
+        repeat econstructor.
+        compat_hsimpl.
+        rewrite NetMod.init_get.
+        eattac.
+      }
+
+      eapply path_seq1 with (act := NComm (Initiator "1" 0) (Worker "endpoint1") Q some_msg).
+      {
+        unfold make_net, my_net_conf, call, recvr, recvq.
+        eapply NComm_neq; eattac.
+        - repeat econstructor.
+          compat_hsimpl in *.
+          eattac.
+        - repeat econstructor.
+          compat_hsimpl in *.
+          rewrite NetMod.init_get.
+          eattac.
+      }
+
+      eapply path_seq1 with (act := NTau (Worker "endpoint1") Tau).
+      {
+        unfold make_net, my_net_conf, call, recvr, recvq.
+        rewrite (unfold_Proc (gen_server _ _)).
+        simpl.
+        repeat econstructor.
+        compat_hsimpl.
+        eattac.
+      }
+
+      eapply path_seq1 with (act := NTau (Worker "endpoint1") Tau).
+      {
+        unfold make_net, my_net_conf, call, recvr, recvq.
+        rewrite (unfold_Proc (run_gen_server _)); simpl.
+        repeat econstructor.
+        compat_hsimpl.
+        eattac.
+      }
+
+      eapply path_seq1 with (act := NComm (Worker "endpoint1") (Worker "proxy0") Q some_msg).
+      {
+        unfold make_net, my_net_conf, call, recvr, recvq.
+        eapply NComm_neq; eattac.
+        - repeat econstructor.
+          compat_hsimpl in *.
+          eattac.
+        - repeat econstructor.
+          compat_hsimpl in *.
+          rewrite NetMod.init_get.
+          eattac.
+      }
+
+      (* Cross *)
+      eapply path_seq1 with (act := NTau (Worker "proxy1") Tau).
+      {
+        unfold make_net, my_net_conf, call, recvr, recvq.
+        rewrite (unfold_Proc (gen_server _ _)).
+        simpl.
+        repeat econstructor.
+        compat_hsimpl.
+        rewrite (unfold_Proc (gen_server _ _)). simpl.
+        eattac.
+      }
+
+      eapply path_seq1 with (act := NTau (Worker "proxy1") Tau).
+      {
+        unfold make_net, my_net_conf, call, recvr, recvq.
+        rewrite (unfold_Proc (run_gen_server _)); simpl.
+        repeat econstructor.
+        compat_hsimpl.
+        eattac.
+      }
+
+      eapply path_seq1 with (act := NComm (Worker "proxy1") (Worker "endpoint1") Q some_msg).
+      {
+        unfold make_net, my_net_conf, call, recvr, recvq.
+        eapply NComm_neq; eattac.
+        - repeat econstructor.
+          compat_hsimpl in *.
+          eattac.
+        - repeat econstructor.
+          compat_hsimpl in *.
+          repeat econstructor.
+      }
+
+      eapply path_seq1 with (act := NTau (Worker "proxy0") Tau).
+      {
+        unfold make_net, my_net_conf, call, recvr, recvq.
+        rewrite (unfold_Proc (gen_server _ _)).
+        simpl.
+        repeat econstructor.
+        compat_hsimpl.
+        eattac.
+      }
+
+      eapply path_seq1 with (act := NTau (Worker "proxy0") Tau).
+      {
+        unfold make_net, my_net_conf, call, recvr, recvq.
+        rewrite (unfold_Proc (run_gen_server _)); simpl.
+        repeat econstructor.
+        compat_hsimpl.
+        eattac.
+      }
+
+      eapply path_seq1 with (act := NComm (Worker "proxy0") (Worker "endpoint0") Q some_msg).
+      {
+        unfold make_net, my_net_conf, call, recvr, recvq.
+        eapply NComm_neq; eattac.
+        - repeat econstructor.
+          compat_hsimpl in *.
+          eattac.
+        - repeat econstructor.
+          compat_hsimpl in *.
+          repeat econstructor.
+      }
+
+      eapply PTnil.
+    }
+
+    match! goal with [_ : _ =[_]=> ?n |- _] => remember $n as N end.
+
+    assert (forall n, Decisive_q (NetMod.get n N)).
+    {
+      enough (forall n, AnySRPC (pq_P (NetMod.get n N))) by (unfold Decisive_q; eauto using SRPC_Decisive).
+      enough (forall n, AnySRPC_pq (NetMod.get n N)) by (intros;
+                                                    destruct `(AnySRPC_pq (NetMod.get n N)) as [srpc ?]; exists srpc;
+                                                    destruct (NetMod.get n N);
+                                                    eauto).
+      enough (SRPC_net N) by eauto.
+      enough (SRPC_net (make_net my_net_conf)) by eauto with LTS.
+      clear.
+      eauto using make_net_SRPC.
+    }
+
+    split; eauto.
+    constructor 1 with (DL:=map Worker ["endpoint0"; "endpoint1"; "proxy0"; "proxy1"]).
+    constructor. 1: { clear; attac. }
+    intros.
+    unfold net_lock.
+    compat_hsimpl.
+    specialize (H0 n).
+    clear H.
+    repeat (destruct `(_ \/ _)).
+    - exists [Worker "proxy1"].
+      subst.
+      compat_hsimpl in *.
+      split; attac.
+      blast_cases. 2: bs.
+      apply NAME.eqb_eq in Heqb.
+      auto.
+    - exists [Worker "proxy0"].
+      subst.
+      compat_hsimpl in *.
+      split; attac.
+      blast_cases. 2: bs.
+      apply NAME.eqb_eq in Heqb.
+      auto.
+    - exists [Worker "endpoint0"].
+      subst.
+      compat_hsimpl in *.
+      split; attac.
+      blast_cases. 2: bs.
+      apply NAME.eqb_eq in Heqb.
+      auto.
+    - exists [Worker "endpoint1"].
+      subst.
+      compat_hsimpl in *.
+      split; attac.
+      blast_cases. 2: bs.
+      apply NAME.eqb_eq in Heqb.
+      auto.
+    - bs.
+  Qed.
+
 End Thomas.
